
<span style='color: blue;'>AI User: Mathematical Analyst</span>


<span style='color: blue;'>Instruction:</span>

<span style='color: blue;'>Start by separating the variables in the given differential equation \( \frac{dy}{dx} = y^2 \sin(x) \).</span>

<span style='color: blue;'>Input:</span>

<span style='color: blue;'>The differential equation \( \frac{dy}{dx} = y^2 \sin(x) \).</span>


<span style='color: darkgreen;'>AI Assistant: Computational Mathematician</span>


<span style='color: darkgreen;'>Solution&amp;Action:</span>

<span style='color: darkgreen;'>The method of separation of variables involves rewriting the equation in a form that shows the product of two functions, each depending only on one of the two variables. In this case, we can rewrite the given differential equation \( \frac{dy}{dx} = y^2 \sin(x) \) as \( \frac{1}{y^2} dy = \sin(x) dx \). </span>


<span style='color: darkgreen;'>This separates the variables y and x on different sides of the equation, with dy and dx representing infinitesimal changes in y and x respectively. The left side of the equation is now a function of y only, and the right side is a function of x only. </span>


<span style='color: darkgreen;'>So, the separated form of the differential equation is \( \frac{1}{y^2} dy = \sin(x) dx \).</span>


<span style='color: blue;'>AI User: Mathematical Analyst</span>


<span style='color: blue;'>Instruction:</span>

<span style='color: blue;'>Now, integrate both sides of the separated differential equation \( \frac{1}{y^2} dy = \sin(x) dx \).</span>

<span style='color: blue;'>Input:</span>

<span style='color: blue;'>The separated differential equation \( \frac{1}{y^2} dy = \sin(x) dx \).</span>


<span style='color: darkgreen;'>AI Assistant: Computational Mathematician</span>


<span style='color: darkgreen;'>Solution&amp;Action:</span>

<span style='color: darkgreen;'>To solve the differential equation, we need to integrate both sides. The integral of \( \frac{1}{y^2} \) with respect to y is \( -\frac{1}{y} \), and the integral of \( \sin(x) \) with respect to x is \( -\cos(x) \).</span>


<span style='color: darkgreen;'>So, the integrated form of the differential equation is \( -\frac{1}{y} = -\cos(x) + C \), where C is the constant of integration.</span>


<span style='color: darkgreen;'>Rearranging the equation gives the general solution of the differential equation as \( y = \frac{1}{\cos(x) - C} \).</span>


<span style='color: blue;'>AI User: Mathematical Analyst</span>


<span style='color: blue;'>Instruction:</span>

<span style='color: blue;'>Now, verify the solution \( y = \frac{1}{\cos(x) - C} \) by substituting it back into the original differential equation \( \frac{dy}{dx} = y^2 \sin(x) \).</span>

<span style='color: blue;'>Input:</span>

<span style='color: blue;'>The original differential equation \( \frac{dy}{dx} = y^2 \sin(x) \) and the general solution \( y = \frac{1}{\cos(x) - C} \).</span>


<span style='color: darkgreen;'>AI Assistant: Computational Mathematician</span>


<span style='color: darkgreen;'>Solution&amp;Action:</span>

<span style='color: darkgreen;'>To verify the solution, we substitute \( y = \frac{1}{\cos(x) - C} \) back into the original differential equation \( \frac{dy}{dx} = y^2 \sin(x) \).</span>


<span style='color: darkgreen;'>First, we need to find the derivative of \( y = \frac{1}{\cos(x) - C} \) with respect to x. Using the chain rule, we get \( \frac{dy}{dx} = \frac{\sin(x)}{(\cos(x) - C)^2} \).</span>


<span style='color: darkgreen;'>Next, we substitute \( y = \frac{1}{\cos(x) - C} \) and \( \frac{dy}{dx} = \frac{\sin(x)}{(\cos(x) - C)^2} \) into the original differential equation \( \frac{dy}{dx} = y^2 \sin(x) \).</span>


<span style='color: darkgreen;'>This gives us \( \frac{\sin(x)}{(\cos(x) - C)^2} = \left(\frac{1}{\cos(x) - C}\right)^2 \sin(x) \).</span>


<span style='color: darkgreen;'>Simplifying the right side of the equation, we get \( \frac{\sin(x)}{(\cos(x) - C)^2} = \frac{\sin(x)}{(\cos(x) - C)^2} \), which verifies that \( y = \frac{1}{\cos(x) - C} \) is indeed a solution to the original differential equation \( \frac{dy}{dx} = y^2 \sin(x) \).</span>


<span style='color: darkgreen;'>So, the solution \( y = \frac{1}{\cos(x) - C} \) has been verified. Next request.</span>


<span style='color: blue;'>AI User: Mathematical Analyst</span>


<span style='color: blue;'>Instruction: </span>

<span style='color: blue;'>CAMEL_TASK_DONE</span>

<span style='color: blue;'>Input: </span>

<span style='color: blue;'>None</span>


<span style='color: darkgreen;'>AI Assistant: Computational Mathematician</span>


<span style='color: darkgreen;'>Solution&amp;Action:</span>

<span style='color: darkgreen;'>Since the task has been marked as completed, no further action is required. Next request.</span>

